tests/lean/run/grind_indexmap.lean
@@ -1,6 +1,8 @@
+module
 -- See also the companion file `grind_indexmap_pre.lean`,
 -- showing this file might have looked like before any proofs are written.
 -- This file fills them all in with `grind`!
+
 import Std.Data.HashMap
 import Lean.LibrarySuggestions.Default
 
@@ -8,6 +10,14 @@ local macro_rules | `(tactic| get_elem_tactic_extensible) => `(tactic| grind)
 
 open Std
 
+/--
+An `IndexMap α β` is a map from keys of type `α` to values of type `β`,
+which also maintains the insertion order of keys.
+
+Internally `IndexMap` is implementented redundantly as a `HashMap` from keys to indices
+(and hence the key type must be `Hashable`), along with `Array`s of keys and values.
+These implementation details are private, and hidden from the user.
+-/
 structure IndexMap (α : Type u) (β : Type v) [BEq α] [Hashable α] where
   private indices : HashMap α Nat
   private keys : Array α
@@ -23,10 +33,11 @@ variable {m : IndexMap α β} {a : α} {b : β} {i : Nat}
 @[inline] def size (m : IndexMap α β) : Nat :=
   m.values.size
 
-attribute [local grind] size
+@[local grind =]
+private theorem size_keys : m.keys.size = m.size := size_keys' _
 
-@[local grind =] private theorem size_keys : m.keys.size = m.size := size_keys' _
-@[local grind =] private theorem size_values : m.values.size = m.size := rfl
+@[local grind =]
+private theorem size_values : m.values.size = m.size := rfl
 
 def emptyWithCapacity (capacity := 8) : IndexMap α β where
   indices := HashMap.emptyWithCapacity capacity
@@ -39,8 +50,7 @@ instance : EmptyCollection (IndexMap α β) where
 instance : Inhabited (IndexMap α β) where
   default := ∅
 
-@[inline] def contains (m : IndexMap α β)
-    (a : α) : Bool :=
+@[inline] def contains (m : IndexMap α β) (a : α) : Bool :=
   m.indices.contains a
 
 instance : Membership α (IndexMap α β) where
@@ -49,7 +59,8 @@ instance : Membership α (IndexMap α β) where
 instance {m : IndexMap α β} {a : α} : Decidable (a ∈ m) :=
   inferInstanceAs (Decidable (a ∈ m.indices))
 
-@[local grind _=_] private theorem mem_indices {m : IndexMap α β} {a : α} :
+@[local grind _=_]
+private theorem mem_indices {m : IndexMap α β} {a : α} :
     a ∈ m.indices ↔ a ∈ m := by rfl
 
 @[inline] def findIdx? (m : IndexMap α β) (a : α) : Option Nat := m.indices[a]?
@@ -66,7 +77,7 @@ variable [LawfulBEq α] [LawfulHashable α]
 attribute [local grind _=_] IndexMap.WF
 
 -- TODO: Considering activating this globally in https://github.com/leanprover/lean4/pull/11963
-grind_pattern getElem?_pos => c[i] where
+local grind_pattern getElem?_pos => c[i] where
   guard dom c i
 
 private theorem getElem_indices_lt {h : a ∈ m} : m.indices[a] < m.size := by
@@ -80,10 +91,14 @@ instance : GetElem? (IndexMap α β) α β (fun m a => a ∈ m) where
   getElem? m a := m.indices[a]?.bind (fun i => (m.values[i]?))
   getElem! m a := m.indices[a]?.bind (fun i => (m.values[i]?)) |>.getD default
 
-@[local grind =] private theorem getElem_def (m : IndexMap α β) (a : α) (h : a ∈ m) : m[a] = m.values[m.indices[a]'h] := rfl
-@[local grind =] private theorem getElem?_def (m : IndexMap α β) (a : α) :
+@[local grind =]
+private theorem getElem_def (m : IndexMap α β) (a : α) (h : a ∈ m) :
+    m[a] = m.values[m.indices[a]'h] := rfl
+@[local grind =]
+private theorem getElem?_def (m : IndexMap α β) (a : α) :
     m[a]? = m.indices[a]?.bind (fun i => (m.values[i]?)) := rfl
-@[local grind =] private theorem getElem!_def [Inhabited β] (m : IndexMap α β) (a : α) :
+@[local grind =]
+private theorem getElem!_def [Inhabited β] (m : IndexMap α β) (a : α) :
     m[a]! = (m.indices[a]?.bind (fun i => (m.values[i]?))).getD default := rfl
 
 instance : LawfulGetElem (IndexMap α β) α β (fun m a => a ∈ m) where
@@ -111,7 +126,9 @@ instance [LawfulBEq α] : Insert (α × β) (IndexMap α β) :=
 instance [LawfulBEq α] : LawfulSingleton (α × β) (IndexMap α β) :=
     ⟨fun _ => rfl⟩
 
-@[local grind .] private theorem WF' (i : Nat) (a : α) (h₁ : i < m.keys.size) (h₂ : a ∈ m) :
+-- This is not needed if we activate `grind_pattern getElem?_pos => c[i]` above.
+@[local grind .]
+private theorem WF' (i : Nat) (a : α) (h₁ : i < m.keys.size) (h₂ : a ∈ m) :
     m.keys[i] = a ↔ m.indices[a] = i := by
   have := m.WF i a
   grind
@@ -137,15 +154,18 @@ If the key is not present, the map is unchanged.
 
 /-! ### Verification theorems -/
 
-@[grind =] theorem mem_insert (m : IndexMap α β) (a a' : α) (b : β) :
+@[grind =]
+theorem mem_insert (m : IndexMap α β) (a a' : α) (b : β) :
     a' ∈ m.insert a b ↔ a' = a ∨ a' ∈ m := by
   grind +locals
 
-@[grind =] theorem getElem_insert (m : IndexMap α β) (a a' : α) (b : β) (h : a' ∈ m.insert a b) :
+@[grind =]
+theorem getElem_insert (m : IndexMap α β) (a a' : α) (b : β) (h : a' ∈ m.insert a b) :
     (m.insert a b)[a'] = if h' : a' == a then b else m[a'] := by
   grind +locals
 
-@[grind =] theorem findIdx_insert_self (m : IndexMap α β) (a : α) (b : β) :
+@[grind =]
+theorem findIdx_insert_self (m : IndexMap α β) (a : α) (b : β) :
     (m.insert a b).findIdx a = if h : a ∈ m then m.findIdx a else m.size := by
   grind +locals
 
@@ -155,7 +175,8 @@ theorem findIdx_lt (m : IndexMap α β) (a : α) (h : a ∈ m) :
 
 grind_pattern findIdx_lt => m.findIdx a h
 
-@[grind =] theorem getIdx_findIdx (m : IndexMap α β) (a : α) (h : a ∈ m) :
+@[grind =]
+theorem getIdx_findIdx (m : IndexMap α β) (a : α) (h : a ∈ m) :
     m.getIdx (m.findIdx a) = m[a] := by grind +locals
 
 end IndexMap
